Test more methods in example

IO/IoNative.cs
@@ -1,70 +1,61 @@
 using System;
-using System.Numerics;
-using System.Diagnostics;
-using System.Threading;
-using System.Collections.Concurrent;
-using System.Collections.Generic;
 using FStream = System.IO.FileStream;
 
 namespace @IoNative {
 
-// public partial class HostConstants
-// {
-//   public static void NumCommandLineArgs(out uint n)
-//   {
-//     n = (uint)System.Environment.GetCommandLineArgs().Length;
-//   }
+public partial class HostConstants
+{
+  public static uint NumCommandLineArgs()
+  {
+    return (uint)System.Environment.GetCommandLineArgs().Length;
+  }
 
-//   public static void GetCommandLineArg(ulong i, out string arg)
-//   {
-//     arg = System.Environment.GetCommandLineArgs()[i];
-//   }
-// }
+  public static char[] GetCommandLineArg(ulong i)
+  {
+    return System.Environment.GetCommandLineArgs()[i].ToCharArray();
+  }
+}
 
 public partial class FileStream
 {
   internal FStream fstream;
   internal FileStream(FStream fstream) { this.fstream = fstream; }
 
-//   public static void FileExists(char[] name, out bool result)
-//   {
-//     result = System.IO.File.Exists(new string(name));      
-//   }
-
-//   public static void FileLength(char[] name, out bool success, out int len)
-//   {
-//     len = 42;
-//     try
-//     {
-//       System.IO.FileInfo fi = new System.IO.FileInfo(new string(name));
-//       if (fi.Length < System.Int32.MaxValue)  // We only support small files
-//       {
-//         len = (int)fi.Length;
-//         success = true;
-//       }
-//       else
-//       {
-//         success = false;
-//       }
+  public static bool FileExists(char[] name)
+  {
+    return System.IO.File.Exists(new string(name));      
+  }
+  
+  public static void FileLength(char[] name, out bool success, out int len)
+  {
+    len = -1;
+    try {
+      System.IO.FileInfo fi = new System.IO.FileInfo(new string(name));
+      if (fi.Length < System.Int32.MaxValue) {  // We only support small files
+        len = (int)fi.Length;
+        success = true;
+      }
+      else {
+        success = false;
+      }
       
-//     }
-//     catch (Exception e)
-//     {
-//       System.Console.Error.WriteLine(e);
-//       success = false;
-//     }     
-//   }
+    }
+    catch (Exception e) {
+      System.Console.Error.WriteLine(e);
+      success = false;
+    }     
+  }
 
   public static void Open(char[] name, out bool ok, out FileStream f)
   {
     try {
-        f = new FileStream(new FStream(new string(name), System.IO.FileMode.OpenOrCreate, System.IO.FileAccess.ReadWrite));
-        ok = true;
+      f = new FileStream(new FStream(new string(name), System.IO.FileMode.OpenOrCreate, System.IO.FileAccess.ReadWrite));
+      ok = true;
     }
     catch (Exception e) {
-        System.Console.Error.WriteLine(e);
-        f = null;
-        ok = false;
+      System.Console.Error.WriteLine(e);
+      f = null;
+      ok = false;
     }
   }
 
