IO/Io.dfy
@@ -4,15 +4,54 @@ module {:extern "IoNative"} Io {
 
   import opened NativeTypes
 
+  //////////////////////////////////////////////////////////////////////////////
+  // Per-host constants
+  //////////////////////////////////////////////////////////////////////////////
+
+  class HostConstants
+  {
+    constructor {:extern} () requires false
+
+    /* Result of C# System.Environment.GetCommandLineArgs(); argument 0 is name
+    of executable. */  
+    function {:extern} CommandLineArgs(): seq<string> reads this
+
+    static method {:extern} NumCommandLineArgs(ghost env: HostEnvironment) returns (n: uint32)
+      ensures n as int == |env.constants.CommandLineArgs()|
+
+    static method {:extern} GetCommandLineArg(i: uint64, ghost env: HostEnvironment) returns (arg: array<char>)
+      requires 0 <= i as int < |env.constants.CommandLineArgs()|
+      ensures  arg[..] == env.constants.CommandLineArgs()[i]
+  }
+
+  //////////////////////////////////////////////////////////////////////////////
+  // Failure
+  //////////////////////////////////////////////////////////////////////////////
+
   class OkState
   {
     constructor {:extern} () requires false
     function {:extern} ok(): bool reads this
   }
 
+  //////////////////////////////////////////////////////////////////////////////
+  // File System
+  //////////////////////////////////////////////////////////////////////////////
+
+  class FileSystemState
+  {
+    constructor {:extern} () requires false
+
+    /* File system maps file names to their contents. */
+    function {:extern} state(): map<string, seq<uint8>>
+      reads this
+  }
+
   class HostEnvironment
   {
+    ghost var constants: HostConstants
     ghost var ok: OkState
+    ghost var files: FileSystemState
   }
 
   class FileStream
@@ -21,6 +60,17 @@ module {:extern "IoNative"} Io {
     function {:extern} Name(): string reads this
     function {:extern} IsOpen(): bool reads this
     constructor {:extern} () requires false
+
+    static method {:extern} FileExists(name: array<char>, ghost env: HostEnvironment) returns (result: bool)
+      requires env.ok.ok()      
+      ensures  result <==> old(name[..]) in env.files.state()      
+
+    static method {:extern} FileLength(name: array<char>, ghost env: HostEnvironment) returns (success: bool, len: int32)
+      requires env.ok.ok()   
+      requires name[..] in env.files.state()
+      modifies env.ok
+      ensures  env.ok.ok() == success
+      ensures  success ==> len as int == |env.files.state()[name[..]]|
 
     static method {:extern} Open(name: array<char>, ghost env: HostEnvironment)
       returns (ok: bool, f: FileStream)
