IO/IoExample.dfy
@@ -6,7 +6,7 @@ module IoExample {
   import opened Io
   import opened NativeTypes
 
-  // Useful to convert Dafny strings into arrays of characters.
+  /* Useful to convert Dafny strings into arrays of characters. */
   method ArrayFromSeq<A>(s: seq<A>) returns (a: array<A>)
     ensures a[..] == s
   {
@@ -20,18 +20,38 @@ module IoExample {
       var fname := ArrayFromSeq("foo.txt");
       var f: FileStream;
       var ok: bool;
+      
+      var numArgs := HostConstants.NumCommandLineArgs(env);
+      if numArgs < 1 {
+        print "Error: invalid number of command line arguments\n";
+        return;
+      }
+      print "# command line args: ";
+      print numArgs;
+      print "\n";
+
+      var arg0 := HostConstants.GetCommandLineArg(0, env);
+      print "command: " + arg0[..] + "\n";
+      
+      var fileExists := FileStream.FileExists(fname, env);
+      if fileExists {
+        print fname[..] + " exists!\n";
+
+        var ok, len := FileStream.FileLength(fname, env);
+        if !ok { print "Error: invalid file length\n"; return; }
+        print fname[..] + " length: ";
+        print len;
+        print "\n";
+      }
+
       ok, f := FileStream.Open(fname, env);
+      if !ok { print "Error: open failed\n"; return; }
 
-      // Try commenting out the following line to see that you are forced to handle errors!
-      if !ok { print "open failed\n"; return; }
-
-      // This is "hello world!" in ascii.
-      // The library requires the data to be an array of bytes, but Dafny has no char->byte conversions :(
+      /* This is "hello world!" in ascii. */
       var data: array<uint8> := ArrayFromSeq([104, 101, 108, 108, 111, 32, 119, 111, 114, 108, 100, 33, 10]);
 
       ok := f.Write(0, data, 0, data.Length as int32);
-
-      if !ok { print "open failed\n"; return; }
+      if !ok { print "Error: write failed\n"; return; }
 
       ok := f.Close();
 
